WIP: Add type `Thing`

Is0.lean
@@ -18,32 +18,53 @@ def State := Std.HashMap String Literal
 
 -- We'll definitely need a context, mapping variable names to values.
 
-inductive Cirgen where
-  | Const : Felt → Cirgen
-  | True : Cirgen
-  | Get : Vector Felt n → Fin n → Felt → Cirgen
-  | Set : Vector Felt n → Fin n → Felt → Cirgen
-  | Sub : Felt → Felt → Cirgen
-  | Mul : Felt → Felt → Cirgen
-  | Isz : Felt → Cirgen
-  | Inv : Felt → Cirgen
-  | AndEqz : Constraint → Felt → Cirgen
-  | AndCond : Constraint → Felt → Constraint → Cirgen
-  | Variable : String → Cirgen
-  | Sequence : Cirgen → Cirgen → Cirgen
-  | Assign : String → Literal → Cirgen
+inductive Thing : Type → Type where
+  | Literal {a} : a → Thing a
+  | Variable {a} : String → Thing a
 
-def Cirgen.step (state : State) (op : Cirgen) : Literal :=
-  match op with
+inductive Expression where
+  | Const : Felt → Expression
+  | True : Expression
+  | Get : Vector Felt n → Fin n → Felt → Expression
+  | Set : Vector Felt n → Fin n → Felt → Expression
+  | Sub : Felt → Felt → Expression
+  | Mul : Felt → Felt → Expression
+  | Isz : Felt → Expression
+  | Inv : Felt → Expression
+  | AndEqz : ConstraintThing → FieldThing → Expression
+  | AndCond : Constraint → Felt → Constraint → Expression
+  | Variable : String → Expression
+
+def Expression.eval (state : State) (e : Expression) : Literal :=
+  match e with
   | Const x => .Val x
   | True => .Constraint (_root_.True)
   | Get buffer i _ => .Val (buffer.get i)
   | Sub x y => .Val (x - y)
-  | Variable name => (state.findD name (Literal.Val 0))
+  | Variable name => state.findD name (Literal.Val 0)
   | AndEqz c x => .Constraint (c ∧ x = 0)
-  | Sequence a b => .Constraint False
-  | Assign name x => state.
   | _ => .Constraint False
 
-open Cirgen in
-theorem Sub_AndEqz_is_if_is_zero : ∀ x : Felt, Sequence (Sub x 1) (AndEqz True state.get "%0") := by sorry
+def Expression.assign (state : State) (e : Expression) (name : String) : State :=
+  state.insert name (Expression.eval state e)
+
+inductive Cirgen where
+  | Sequence : Cirgen → Cirgen → Cirgen
+  | Assign : String → Expression → Cirgen
+  -- Should this take a String?
+  | Return : Expression → Cirgen
+
+def Cirgen.step (state : State) (op : Cirgen) : State × Option Literal :=
+  match op with
+  -- We may want to encode the index of the instruction in `State`, and then
+  -- always assign to the index instead of using a name.
+  | Assign e name => (Expression.assign state e name, none)
+  | Sequence a b => let (state', x) := Cirgen.step state a
+                    match x with
+                    | some x => (state', some x)
+                    | none => Cirgen.step state' b
+  | Return e => (state, Expression.eval state e)
+
+open Expression Cirgen in
+theorem Sub_AndEqz_is_if_is_zero (state : State) :
+  ∀ x : Felt, Sequence (Assign "x-1" (Expression.Sub x 1)) (Assign "(x-1)=0" (AndEqz True (Variable "x-1"))) := by sorry
